\chapter{Proof of Proposition~\ref{prop:opred}}\label{app:opred}
Given $I(x)$ a candidate index function we associate the point-like measure
\[
p_i(x) = \delta_{i,I(x)}.
\]
Written in terms of $p$ the loss function reads
\[
{\cal L}_2(\hat y,p) = {\mathbb E}_{x,{\bf y}}\Bigl[\sum_{i\in T} p_i(x)\bigl(y_i-\hat y(x)\bigr)^2\Bigr].
\]
%Under~(\ref{eq:py}) (with $\alpha_{ij}=\alpha\delta_{ij}$) the loss is equal to
Under~(3) (with $\alpha_{ij}=\alpha\delta_{ij}$) the loss is equal to
\[
{\cal L}_2(\hat y,p) = {\mathbb E}_x\Bigl[\sum_{i\in T} p_i(x)\Bigl( \bigl(\hat y_i(x)-\hat y(x)\bigr)^2-\hat p_i(x)\frac{\alpha\sigma^2}{1+\alpha}\Bigr)\Bigr]+\sigma^2
\]
The minimization w.r.t. $\hat y$ yields
\begin{equation}\label{eq:hy}
\hat y(x) = \sum_{i\in T} p_i(x)\hat y_i(x).
\end{equation}
In turn, as a function of $p_i$ the loss being a  convex combination, its minimization yields
\begin{align}
  p_i(x) &= \delta_{i,I(x)},\label{eq:hp}\\[0.2cm]
  I(x) &= \argmin_{i\in T}\Bigl(\bigl(\hat y_i(x)-\hat y(x)\bigr)^2-\hat p_i(x)\frac{\alpha\sigma^2}{1+\alpha}\Bigr).\label{eq:hI}
\end{align}
Combining these equations~(\ref{eq:hy},\ref{eq:hp},\ref{eq:hI}) we get
\[
I(x) = \argmax_{i\in T}\bigl(\hat p_i(x)\bigr),
\]
which concludes the proof.  
